WIP

src/axiomatic/Gevents.v
@@ -9,367 +9,128 @@ Require Import Basic Event.
 
 Set Implicit Arguments.
 
-(** * Labels *)
+Definition act_id := nat.
+Definition thread_id := IdentMap.key.
 
 Inductive label := 
-(*  | Askip*)
-  | Aload   (loc:Loc.t) (val:Const.t) (ord:Ordering.t)
-  | Astore  (loc:Loc.t) (val:Const.t) (ord:Ordering.t)
-  | Arfence (ord:Ordering.t)
-  | Awfence (ord:Ordering.t).
+  | Aload (l:Loc.t) (v:Const.t) (o:Ordering.t)
+  | Astore (l:Loc.t) (v:Const.t) (o:Ordering.t)
+  | Arfence (o:Ordering.t)
+  | Awfence (o:Ordering.t).
 
-Definition loc_lab a :=
+Inductive event := 
+  | Event (id: act_id) (tid: thread_id) (lb:label).
+
+Definition id a :=
   match a with
-(*  | Askip  => None*)
-  | Aload  l _ _
-  | Astore l _ _ => Some l
-  | Arfence _ 
-  | Awfence _ => None
+  | Event  id _ _ => id
   end.
 
-Definition val_lab a :=
+Definition thread a :=
   match a with
-(*  | Askip  => None*)
+  | Event  _ i _ => i
+  end.
+
+Definition lab a :=
+  match a with
+  | Event  _ _ lb => lb
+  end.
+
+Definition loc a :=
+  match (lab a) with
+  | Aload l _ _
+  | Astore l _ _ => Some l
+  | _ => None
+  end.
+
+Definition val a :=
+  match (lab a) with
   | Aload  _ v _
   | Astore _ v _ => Some v
-  | Arfence _ 
-  | Awfence _ => None
+  | _ => None
   end.
 
-Definition ord_lab a :=
-  match a with
-(*  | Askip  => None*)
+Definition ord a :=
+  match (lab a) with
   | Aload  _ _ o
   | Astore _ _ o
   | Arfence o 
   | Awfence o => o
   end.
 
-Definition is_read_lab a :=
-  match a with
-    | Aload _ _ _ => True
-    | _ => False
+Definition is_read a := 
+  match (lab a) with
+  | Aload  _ _ _ => True
+  | _ => False
   end.
 
-Definition is_write_lab a :=
-  match a with
-    | Astore  _ _ _ => True
-    | _ => False
+Definition is_write a := 
+  match (lab a) with
+  | Astore _ _ _ => True
+  | _ => False
   end.
 
-Definition is_wfence_lab a :=
-  match a with
-    | Awfence _ => True
-    | _ => False
+Definition is_rfence a := 
+  match (lab a) with
+  | Arfence _ => True
+  | _ => False
   end.
 
-Definition is_rfence_lab a :=
-  match a with
-    | Arfence _ => True
-    | _ => False
+Definition is_wfence a := 
+  match (lab a) with
+  | Awfence  _ => True
+  | _ => False
   end.
 
-Definition is_rlx_lab a :Prop := Ordering.le Ordering.relaxed (ord_lab a).
-Definition is_ra_lab a :Prop := Ordering.le Ordering.acqrel (ord_lab a).
-Definition is_sc_lab a :Prop := Ordering.le Ordering.seqcst (ord_lab a).
-
-(** * Events *)
-Definition act_id := nat.
-Definition thread_id := IdentMap.key.
-
-Inductive event := 
-  | Event (id: act_id) (tid: thread_id) (lab:label).
-
-Definition thread a :=
-  match a with
-  | Event _ tid _ => tid
-  end.
-
-Definition lab a :=
-  match a with
-  | Event _ _ lab => lab
-  end.
-
-Definition loc a := loc_lab (lab a).
-Definition val a := val_lab (lab a).
-Definition ord a := ord_lab (lab a).
-Definition is_read a := is_read_lab (lab a).
-Definition is_write a := is_write_lab (lab a).
-Definition is_wfence a := is_wfence_lab (lab a).
-Definition is_rfence a := is_rfence_lab (lab a).
-Definition is_rlx a :Prop := is_rlx_lab (lab a).
-Definition is_ra a :Prop := is_ra_lab (lab a).
-Definition is_sc a :Prop := is_sc_lab (lab a).
+Definition is_rlx a :Prop := Ordering.le Ordering.relaxed (ord a).
+Definition is_ra  a :Prop := Ordering.le Ordering.acqrel  (ord a).
+Definition is_sc  a :Prop := Ordering.le Ordering.seqcst  (ord a).
 
 (** * Basic Lemmas *)
 
+Lemma read_non_write a (A: is_read a) : ~ is_write a.
+Proof. destruct a; destruct lb; ins. Qed.
 Lemma write_non_read a (A: is_write a) : ~ is_read a.
-Proof.
-unfold is_write, is_read in *.
-destruct a; destruct lab0; ins; eexists; desf; eauto.
-Qed.
-
+Proof. destruct a; destruct lb; ins. Qed.
 Lemma wfence_non_read a (A: is_wfence a) : ~ is_read a.
-Proof.
-unfold is_wfence, is_read in *.
-destruct a; destruct lab0; ins; eexists; desf; eauto.
-Qed.
+Proof. destruct a; destruct lb; ins. Qed.
+Lemma write_non_rfence a (A: is_write a) : ~ is_rfence a.
+Proof. destruct a; destruct lb; ins. Qed.
+Lemma write_non_wfence a (A: is_write a) : ~ is_wfence a.
+Proof. destruct a; destruct lb; ins. Qed.
 
-Lemma write_has_location a (WRITE: is_write a) : exists x, loc a = Some x.
-Proof.
-destruct a; destruct lab0; ins; eexists; desf; eauto.
-Qed.
 
+Lemma write_has_location a (WRITE: is_write a) : exists l, loc a = Some l.
+Proof. unfold loc; destruct a; destruct lb; ins; eauto. Qed.
 Lemma ra_is_rlx a (RA: is_ra a) : is_rlx a.
-Proof.
-destruct a; destruct lab0; ins; desf;  destruct ord0; ins; desf.
-Qed.
-
+Proof. destruct a; destruct lb; destruct o; ins. Qed.
 Lemma sc_is_rlx a (SC: is_sc a) : is_rlx a.
-Proof.
-destruct a; destruct lab0; ins; desf;  destruct ord0; ins; desf.
-Qed.
-
+Proof. destruct a; destruct lb; destruct o; ins. Qed.
 Lemma sc_is_ra a (SC: is_sc a) : is_ra a.
-Proof.
-destruct a; destruct lab0; ins; desf;  destruct ord0; ins; desf.
-Qed.
+Proof. destruct a; destruct lb; destruct o; ins. Qed.
 
-Hint Resolve  write_non_read wfence_non_read ra_is_rlx sc_is_rlx sc_is_ra : acts.
+Lemma read_is_read a l v o (A: lab a = Aload l v o) : is_read a.
+Proof. destruct a; destruct lb; ins. Qed.
+Lemma write_is_write a l v o (A: lab a = Astore l v o) : is_write a.
+Proof. destruct a; destruct lb; ins. Qed.
 
-(*
-Definition is_access a :=
-  match a with
-    | Aload _ _ _ _ | Astore _ _ _ _ | Armw _ _ _ _ _  => true
-    | Askip _ => false
-  end.
+Lemma read_rlx a l v o (A: lab a = Aload l v o) : Ordering.le Ordering.relaxed o -> is_rlx a.
+Proof. unfold is_rlx; unfold ord; rewrite A; done. Qed.
+Lemma read_ra a l v o (A: lab a = Aload l v o) : Ordering.le Ordering.acqrel o -> is_ra a.
+Proof. unfold is_ra; unfold ord; rewrite A; done. Qed.
+Lemma read_sc a l v o (A: lab a = Aload l v o) : Ordering.le Ordering.seqcst o -> is_sc a.
+Proof. unfold is_sc; unfold ord; rewrite A; done. Qed.
 
-(** A read is either a load or a read-modify-write action. *)
-
-Definition is_read a :=
-  match a with
-    | Aload _ _ _ _ | Armw _ _ _ _ _  => true
-    | _ => false
-  end.
-
-Definition is_readL a l :=
-  match a with
-    | Aload _ _ l' _
-    | Armw _ _ l' _ _ => l' = l
-    | _ => False
-  end.
-
-Definition is_readLV a l v :=
-  match a with
-    | Aload _ _ l' v' 
-    | Armw _ _ l' v' _ => l' = l /\ v' = v
-    | _ => False
-  end.
-
-Definition is_read_only a :=
-  match a with
-    | Askip _ => false
-    | Aload _ _ _ _ => true
-    | Armw _ _ _ _ _ => false
-    | Astore _ _ _ _ => false
-  end.
-
-(** A write is either a store or a read-modify-write action. *)
-
-Definition is_write a :=
-  match a with
-    | Astore _ _ _ _ | Armw _ _ _ _ _ => true
-    | _ => false
-  end.
-
-Definition is_writeL a l :=
-  match a with
-    | Astore _ _ l' _ 
-    | Armw _ _ l' _ _ => l' = l
-    | _ => False
-  end.
-
-Definition is_writeLV a l v :=
-  match a with
-    | Astore _ _ l' v' 
-    | Armw _ _ l' _ v' => l' = l /\ v' = v
-    | _ => False
-  end.
-
-Definition is_write_only a :=
-    match a with
-    | Askip _       => false
-    | Aload _ _ _ _ => false
-    | Armw _ _ _ _ _ => false
-    | Astore _ _ _ _ => true
-  end.
-
-Definition is_rmw a :=
-  match a with
-    | Armw _ _ _ _ _ => true
-    | _ => false
-  end.
-
-Lemma is_rmwE a : is_rmw a <-> is_read a /\ is_write a.
-Proof. destruct a; ins; intuition. Qed.
-
-  
-(** Acquire actions have memory order [acq] or stronger. *)
- 
-Definition is_acquire_rtyp t :=
-   match t with RATacq => true end.
-
-Definition is_acquire_utyp t :=
-   match t with UATrel_acq => true end.
-
-Definition is_acquire a :=
-  match a with
-    | Aload _ typ _ _ => is_acquire_rtyp typ
-    | Armw  _ typ _ _ _ => is_acquire_utyp typ
-    | _ => false
-  end.
-
-(** Release actions have memory order [rel] or stronger. *)
-
-Definition is_release_wtyp t :=
-   match t with WATrel => true end.
-
-Definition is_release_utyp t :=
-   match t with | UATrel_acq => true end.
-
-Definition is_release_write a :=
-  match a with
-    | Astore _ typ _ _ => is_release_wtyp typ 
-    | Armw   _ typ _ _ _ => is_release_utyp typ
-    | _ => false
-  end.
+Lemma write_rlx a l v o (A: lab a = Astore l v o) : Ordering.le Ordering.relaxed o -> is_rlx a.
+Proof. unfold is_rlx; unfold ord; rewrite A; done. Qed.
+Lemma write_ra a l v o (A: lab a = Astore l v o) : Ordering.le Ordering.acqrel o -> is_ra a.
+Proof. unfold is_ra; unfold ord; rewrite A; done. Qed.
+Lemma write_sc a l v o (A: lab a = Astore l v o) : Ordering.le Ordering.seqcst o -> is_sc a.
+Proof. unfold is_sc; unfold ord; rewrite A; done. Qed.
 
 
-(******************************************************************************)
-(** ** Lemmas about access types *)
-(******************************************************************************)
+Hint Resolve  read_non_write write_non_read wfence_non_read ra_is_rlx 
+sc_is_rlx sc_is_ra read_is_read read_rlx read_ra read_sc
+write_is_write write_rlx write_ra write_sc 
+write_non_rfence write_non_wfence : acts.
 
-Lemma is_readLV_rmw_writeL a l v : is_readLV a l v -> is_rmw a -> is_writeL a l.
-Proof. by destruct a; ins; desf. Qed.
-
-Lemma is_readL_rmw_writeL a l : is_readL a l -> is_rmw a -> is_writeL a l.
-Proof. by destruct a; ins; desf. Qed.
-
-Lemma is_writeLV_writeL a l v : is_writeLV a l v -> is_writeL a l.
-Proof. by destruct a; ins; desf. Qed.
-
-(** Lemmas deriving [is_readL]. *)
-
-Lemma is_writeLV_rmw_readL a l v : is_writeLV a l v -> is_rmw a -> is_readL a l.
-Proof. by destruct a; ins; desf. Qed.
-
-Lemma is_writeL_rmw_readL a l : is_writeL a l -> is_rmw a -> is_readL a l.
-Proof. by destruct a; ins; desf. Qed.
-
-Lemma is_readLV_readL a l v : is_readLV a l v -> is_readL a l.
-Proof. by destruct a; ins; desf. Qed.
-
-(** Lemmas deriving [is_write]. *)
-
-Lemma is_rmw_write : 
-  forall a, is_rmw a -> is_write a.
-Proof. by destruct a; ins; desf. Qed.
-
-Lemma is_writeLV_write : 
-  forall a l v, is_writeLV a l v -> is_write a.
-Proof. by destruct a; ins; desf. Qed.
-
-Lemma is_writeL_write : 
-  forall a l, is_writeL a l -> is_write a.
-Proof. by destruct a; ins; desf. Qed.
-
-Lemma is_release_write_write : 
-  forall a, is_release_write a -> is_write a.
-Proof. by destruct a; ins; desf. Qed.
-
-(** Lemmas deriving [is_read]. *)
-
-Lemma is_rmw_read : 
-  forall a, is_rmw a -> is_read a.
-Proof. by destruct a; ins; desf. Qed.
-
-Lemma is_readLV_read : 
-  forall a l v, is_readLV a l v -> is_read a.
-Proof. by destruct a; ins; desf. Qed.
-
-Lemma is_readL_read : 
-  forall a l, is_readL a l -> is_read a.
-Proof. by destruct a; ins; desf. Qed.
-
-Lemma is_readL_loc : forall x l, is_readL x l ->
-                                 loc x = l.
-Proof. by destruct x; ins; desf. Qed.
-
-Lemma is_writeL_loc : forall x l, is_writeL x l ->
-                                  loc x = l.
-Proof. by destruct x; ins; desf. Qed.
-
-Lemma is_readLV_loc : forall x l v, is_readLV x l v ->
-                                    loc x = l.
-Proof. by destruct x; ins; desf. Qed.
-      
-Lemma is_writeLV_loc : forall x l v, is_writeLV x l v ->
-                                     loc x = l.
-Proof. by destruct x; ins; desf. Qed.
-
-
-Lemma is_write_write_only : forall x, is_write_only x = true ->
-                                      is_write x = true.
-Proof.
-  ins; destruct x; simpl in *; auto.
-Qed.
-
-Lemma is_read_read_only : forall x, is_read_only x = true ->
-                                      is_read x = true.
-Proof.
-  ins; destruct x; simpl in *; auto.
-Qed.
-  
-Hint Resolve
-  is_writeLV_writeL    is_readLV_readL
-  is_writeL_write      is_writeLV_write    is_rmw_write
-  is_readL_read        is_readLV_read      is_rmw_read
-  is_readL_loc is_writeL_loc
-  is_readLV_loc is_writeLV_loc : caccess.
-
-
-Lemma is_write_access a : is_write a -> is_access a.
-Proof. by destruct a. Qed.
-
-Lemma is_read_access a : is_read a -> is_access a.
-Proof. by destruct a. Qed.
-
-Lemma is_writeL_access a l : is_writeL a l -> is_access a.
-Proof. by destruct a. Qed.
-
-Lemma is_readL_access a l : is_readL a l -> is_access a.
-Proof. by destruct a. Qed.
-
-Lemma is_readLV_access a l v : is_readLV a l v -> is_access a.
-Proof. by destruct a. Qed.
-
-Hint Resolve is_read_access is_readL_access is_readLV_access
-             is_write_access is_writeL_access : caccess.
-
-Lemma is_read_only_access a : is_read_only a -> is_access a.
-Proof. by destruct a. Qed.
-
-Lemma is_write_only_access a : is_write_only a -> is_access a.
-Proof. by destruct a. Qed.
-
-Lemma is_read_only_read a : is_read_only a -> is_read a.
-Proof. by destruct a. Qed.
-
-Lemma is_write_only_write a : is_write_only a -> is_write a.
-Proof. by destruct a. Qed.
-
-Hint Resolve is_read_only_read is_read_only_access
-     is_write_only_write is_write_only_access : caccess.
-
-
-*)
