src/axiomatic/Machine.v
@@ -37,19 +37,54 @@ Record configuration :=
     mo : event -> event -> Prop ; 
     sc : event -> event -> Prop }.
 
-(*Definition Coherent_configuration (mc : configuration) := 
-  Coherent (Macts mc) (Mlab mc) (Msb mc) (Mrmw mc) (Mrf mc) (Mmo mc) (Msc mc).*)
+Definition id_gstep mc mc' : Prop :=
+  << SAME_ACTS: acts mc = acts mc' >> /\
+  << SAME_SB: sb mc = sb mc' >> /\
+  << SAME_RMW: rmw mc = rmw mc' >> /\
+  << SAME_RF: rf mc = rf mc' >> /\
+  << SAME_MO: mo mc = mo mc' >> /\
+  << SAME_SC: sc mc = sc mc' >>.
 
-Inductive m_step (mc mc' : configuration) : Prop :=
-  | Mstep_read lang  st st' a l v o
-      (TID: IdentMap.find (thread a) (ts mc) = Some (existT _ lang st))
-      (STATE: lang.(Language.step) (Some (ProgramEvent.read l v o)) st st')
-      (MTS: ts mc' = IdentMap.add (thread a) (existT _ _ st') (ts mc))
-      (LAB_STEP: lab a = (Aload l v o))
+Inductive mstep mc mc' e i : Prop :=
+  | silent (SILENT: e = None) (ID_GRAPH: id_gstep mc mc')
+  | read a l v o 
+      (EVENT: e = Some (ProgramEvent.read l v o)) 
+      (LABa: lab a = Aload l v o) 
+      (TIDa: thread a = i) 
       (GSTEP: gstep (acts mc) (sb mc) (rmw mc) (rf mc) (mo mc) (sc mc)
-                         (acts mc') (sb mc') (rmw mc') (rf mc') (mo mc') (sc mc') a).
-(* TODO: add more steps *)
+                    (acts mc') (sb mc') (rmw mc') (rf mc') (mo mc') (sc mc') a)
+  | write a l v o 
+      (EVENT: e = Some (ProgramEvent.write l v o)) 
+      (LABa: lab a = Astore l v o) 
+      (TIDa: thread a = i) 
+      (GSTEP: gstep (acts mc) (sb mc) (rmw mc) (rf mc) (mo mc) (sc mc)
+                    (acts mc') (sb mc') (rmw mc') (rf mc') (mo mc') (sc mc') a)
+  | update a_r a_w l v_r v_w o_r o_w 
+      (EVENT: e = Some (ProgramEvent.update l v_r v_w o_r o_w)) 
+      (LABar: lab a_r = Aload l v_r o_r) (LABaw: lab a_w = Astore l v_w o_w) 
+      (TIDar: thread a_r = i) (TIDaw: thread a_w = i) 
+      mc_mid
+      (GSTEPr: gstep (acts mc) (sb mc) (rmw mc) (rf mc) (mo mc) (sc mc)
+           (acts mc_mid) (sb mc_mid) (rmw mc_mid) (rf mc_mid) (mo mc_mid) (sc mc_mid) a_r)
+      (GSTEPw: gstep (acts mc_mid) (sb mc_mid) (rmw mc_mid) (rf mc_mid) (mo mc_mid) (sc mc_mid)
+                     (acts mc') (sb mc') (rmw mc') (rf mc') (mo mc') (sc mc') a_w)
+  | fence a_r a_w o_r o_w (EVENT: e = Some (ProgramEvent.fence o_r o_w)) 
+      (LABar: lab a_r = Arfence o_r) (LABaw: lab a_w = Awfence o_w) 
+      (TIDar: thread a_r = i) (TIDaw: thread a_w = i) 
+      mc_mid
+      (GSTEPr: gstep (acts mc) (sb mc) (rmw mc) (rf mc) (mo mc) (sc mc)
+           (acts mc_mid) (sb mc_mid) (rmw mc_mid) (rf mc_mid) (mo mc_mid) (sc mc_mid) a_r)
+      (GSTEPw: gstep (acts mc_mid) (sb mc_mid) (rmw mc_mid) (rf mc_mid) (mo mc_mid) (sc mc_mid)
+                     (acts mc') (sb mc') (rmw mc') (rf mc') (mo mc') (sc mc') a_w).
 
+Inductive step mc mc' : Prop :=
+| step_intro  
+    lang st st' i e
+    (TID: IdentMap.find i (ts mc) = Some (existT _ lang st))
+    (STATE: lang.(Language.step) e st st')
+    (MTS: ts mc' = IdentMap.add i (existT _ _ st') (ts mc))
+    (MSTEP: mstep mc mc' e i)
+.
 
 End Operational.
 
