src/axiomatic/sim.v
@@ -29,6 +29,51 @@ Remove Hints plus_n_O.
 
 Hint Resolve gstep_coh gstep_inc coh_wf.
 
+Section Monotone.
+
+Definition monotone (mo : event -> event -> Prop) f :=
+  forall a b, mo a b -> Time.lt (f a) (f b).
+
+Lemma new_f acts sb rmw rf mo sc acts' sb' rmw' rf' mo' sc'
+  a (GSTEP: gstep acts sb rmw rf mo sc acts' sb' rmw' rf' mo' sc' a)
+  f (MON: monotone mo f): 
+  exists f', << F: forall b, In b acts -> f' b = f b >> /\
+             << MON: monotone mo' f' >>.
+Admitted.
+
+Lemma monotone_converse a b l f acts mo
+  (INa: In a acts) (INb: In b acts) (WRITEa: is_write a) (WRITEb: is_write b)
+  (LOCa: loc a = Some l) (LOCb: loc b = Some l) (MON: monotone mo f)
+  (WF_MO: WfMO acts mo) (NOMO: ~ mo b a): Time.le (f a) (f b).
+Proof.
+apply Time.le_lteq.
+destruct (classic (a=b)) as [|N]; desf; eauto.
+eapply WF_MO in N; desf; eauto.
+Qed.
+
+Lemma monotone_converse_strict a b l f acts mo
+  (INa: In a acts) (INb: In b acts) (WRITEa: is_write a) (WRITEb: is_write b)
+  (LOCa: loc a = Some l) (LOCb: loc b = Some l) (MON: monotone mo f)
+  (WF_MO: WfMO acts mo) (NOMO: ~ mo b a) (NEQ: a <> b) : Time.lt (f a) (f b).
+Proof.
+assert (mo a b).
+  eapply wf_mo_tot; eauto.
+apply MON; done.
+Qed.
+
+Definition max_value f (INR : event -> Prop) val :=
+ << UB: forall a (INa: INR a), Time.le (f a) val >> /\
+ << MAX: exists a_max, << INa: INR a_max >> /\ <<LB': Time.le val (f a_max)>> >>.
+
+End Monotone.
+
+Require Import Setoid Permutation.
+
+Add Parametric Morphism : (monotone) with signature 
+  same_relation ==> eq ==> iff as monotone_more.
+Proof.
+  unfold monotone, same_relation, NW; intuition; eauto. 
+Qed.
 
 Section Simulation.
 
@@ -41,34 +86,16 @@ Variable rf : event -> event -> Prop.
 Variable mo : event -> event -> Prop. 
 Variable sc : event -> event -> Prop. 
 
-Definition f_equal_max (INR : event -> Prop) val :=
- << UB: forall a (INa: INR a), Time.le (f a) val >> /\
- << MAX: exists a_max, << INa: INR a_max >> /\ <<LB': Time.le val (f a_max)>> >>.
- 
-Definition valid :=
-  forall a b, mo a b -> Time.lt (f a) (f b).
-
-Lemma valid_converse a b l 
-  (INa: In a acts) (INb: In b acts) (WRITEa: is_write a) (WRITEb: is_write b)
-  (LOCa: loc a = Some l) (LOCb: loc b = Some l) (VALID: valid)
-  (TOT_MO: forall l, is_total (fun a => (In a acts) /\ is_write a /\ loc a = Some l) mo)
-  (NOMO: ~ mo b a): Time.le (f a) (f b).
-Proof.
-apply Time.le_lteq.
-destruct (classic (a=b)) as [|N]; desf; eauto.
-eapply TOT_MO in N; desf; eauto.
-Qed.
-
 Definition sim_msg (m: Message.t) b:=
   << VAL: Some m.(Message.val) = (val b) >> /\
-  << UR: forall l, f_equal_max (msg_rel urr acts sb rmw rf sc l b) ((m.(Message.released)).(Capability.ur) l) >> /\
-  << RW: forall l, f_equal_max (msg_rel rwr acts sb rmw rf sc l b) ((m.(Message.released)).(Capability.rw) l) >> /\
-  << SC: forall l, f_equal_max (msg_rel scr acts sb rmw rf sc l b) ((m.(Message.released)).(Capability.sc) l) >>.
+  << UR: forall l, max_value f (fun a => msg_rel urr acts sb rmw rf sc l a b) ((m.(Message.released)).(Capability.ur) l) >> /\
+  << RW: forall l, max_value f (fun a => msg_rel rwr acts sb rmw rf sc l a b) ((m.(Message.released)).(Capability.rw) l) >> /\
+  << SC: forall l, max_value f (fun a => msg_rel scr acts sb rmw rf sc l a b) ((m.(Message.released)).(Capability.sc) l) >>.
 
 Definition sim_cell_helper b from msg :=
   << SIMMSG: sim_msg msg b >> /\ 
   << FROM: Time.lt from (f b) >> /\ 
-  << FROMRMW: (forall a (RFRMW: (seq rf rmw) a b), from = f a) >>.
+  << FROMRMW: (forall a (RFRMW: (rf ;; rmw) a b), from = f a) >>.
 
 Definition sim_cell cell l  :=
   << DOM: forall b, (is_write b) /\ (loc b = Some l) <-> Cell.get (f b) cell <> None >> /\
@@ -80,19 +107,19 @@ Definition sim_mem (mem: Memory.t) :=
   forall l, sim_cell (mem l) l.
 
 Definition sim_rel rel i :=
-  << REL_UR: forall l' l, f_equal_max (t_rel urr acts sb rmw rf sc i l' l) ((rel l').(Capability.ur) l) >> /\
-  << REL_RW: forall l' l, f_equal_max (t_rel rwr acts sb rmw rf sc i l' l) ((rel l').(Capability.rw) l) >> /\
-  << REL_SC: forall l' l, f_equal_max (t_rel scr acts sb rmw rf sc i l' l) ((rel l').(Capability.sc) l) >>.
+  << REL_UR: forall l' l, max_value f (t_rel urr acts sb rmw rf sc i l' l) ((rel l').(Capability.ur) l) >> /\
+  << REL_RW: forall l' l, max_value f (t_rel rwr acts sb rmw rf sc i l' l) ((rel l').(Capability.rw) l) >> /\
+  << REL_SC: forall l' l, max_value f (t_rel scr acts sb rmw rf sc i l' l) ((rel l').(Capability.sc) l) >>.
 
 Definition sim_cur cur i :=
-  << CUR_UR: forall l, f_equal_max (t_cur urr acts sb rmw rf sc i l) (cur.(Capability.ur) l) >> /\
-  << CUR_RW: forall l, f_equal_max (t_cur rwr acts sb rmw rf sc i l) (cur.(Capability.rw) l) >> /\
-  << CUR_SC: forall l, f_equal_max (t_cur scr acts sb rmw rf sc i l) (cur.(Capability.sc) l) >>.
+  << CUR_UR: forall l, max_value f (t_cur urr acts sb rmw rf sc i l) (cur.(Capability.ur) l) >> /\
+  << CUR_RW: forall l, max_value f (t_cur rwr acts sb rmw rf sc i l) (cur.(Capability.rw) l) >> /\
+  << CUR_SC: forall l, max_value f (t_cur scr acts sb rmw rf sc i l) (cur.(Capability.sc) l) >>.
 
 Definition sim_acq acq i :=
-  << ACQ_UR: forall l, f_equal_max (t_acq urr acts sb rmw rf sc i l) (acq.(Capability.ur) l) >> /\
-  << ACQ_RW: forall l, f_equal_max (t_acq rwr acts sb rmw rf sc i l) (acq.(Capability.rw) l) >> /\
-  << ACQ_SC: forall l, f_equal_max (t_acq scr acts sb rmw rf sc i l) (acq.(Capability.sc) l) >>.
+  << ACQ_UR: forall l, max_value f (t_acq urr acts sb rmw rf sc i l) (acq.(Capability.ur) l) >> /\
+  << ACQ_RW: forall l, max_value f (t_acq rwr acts sb rmw rf sc i l) (acq.(Capability.rw) l) >> /\
+  << ACQ_SC: forall l, max_value f (t_acq scr acts sb rmw rf sc i l) (acq.(Capability.sc) l) >>.
 
 Definition sim_commit commit i :=
   << CUR: sim_cur commit.(Commit.cur) i >> /\
@@ -104,20 +131,10 @@ Definition sim_local local i :=
 
 End Simulation.
 
-Require Import Setoid Permutation.
-
-Add Parametric Morphism : (valid) with signature 
-  eq ==> same_relation ==> iff as valid_more.
-Proof.
-  unfold valid, same_relation, NW; intuition; eauto. 
-Qed.
-
-
-
 Definition sim_f f (op_st: Configuration.t) (ax_st: Machine.configuration) :=
   << LOCAL: forall i foo local (TID: IdentMap.find i (Configuration.threads op_st) = Some (foo, local)),
                 sim_local f (acts ax_st) (sb ax_st) (rmw ax_st) (rf ax_st) (sc ax_st) local i >> /\
-  << SC: forall l, f_equal_max f (S_tm (acts ax_st) (sb ax_st) (rmw ax_st) (rf ax_st) l) (Configuration.sc op_st l)  >> /\
+  << SC: forall l, max_value f (S_tm (acts ax_st) (sb ax_st) (rmw ax_st) (rf ax_st) l) (Configuration.sc op_st l)  >> /\
   << MEM: sim_mem f (acts ax_st) (sb ax_st) (rmw ax_st) (rf ax_st) (sc ax_st) op_st.(Configuration.memory) >>.
 
 Definition sim (op_st: Configuration.t) (ax_st: Machine.configuration) :=
@@ -127,7 +144,7 @@ Definition sim (op_st: Configuration.t) (ax_st: Machine.configuration) :=
   << NO_PROMISES: forall i foo local (TID: IdentMap.find i (Configuration.threads op_st) = Some (foo, local)),
          local.(Local.promises) = Memory.bot>> /\
   << STATES: ts ax_st = IdentMap.map fst (Configuration.threads op_st) >> /\
-  << TIME: exists f, << MONOTONE: valid f (mo ax_st) >> /\  << SIM: sim_f f op_st ax_st >>>>.
+  << TIME: exists f, << MONOTONE: monotone (mo ax_st) f >> /\  << SIM: sim_f f op_st ax_st >>>>.
 
 Lemma find_mapD A B tid (f: A -> B) x y :
   IdentMap.find tid (IdentMap.map f x) = Some y ->
@@ -173,6 +190,10 @@ Lemma if_arg
   (if b then fT else fF) x = if b then fT x else fF x.
 Proof. by case b. Qed.
 
+Lemma if_same 
+(A : Type) (b : bool): forall f : A,
+  (if b then f else f) = f.
+Proof. desf. Qed.
 
 Lemma tm_join a b l :
   TimeMap.join a b l =  Time.join (a l) (b l).
@@ -217,73 +238,84 @@ apply TimeMap.bot_spec.
 apply TimeMap.join_l.
 Qed.
 
-Lemma f_equal_max_singleton f b :
-  f_equal_max f (eq b) (f b).
+Lemma max_value_singleton f b t (T: t = f b):
+  max_value f (eq b) t.
 Proof.
 red; splits; ins; desc; subst.
 by apply Time.le_lteq; eauto.
 exists b; splits; try apply Time.le_lteq; eauto.
 Qed.
 
+Lemma max_value_same_set f f' P P' t :
+  max_value f P t ->
+  (forall x, P x <-> P' x) ->  
+  (forall x, P x -> f' x = f x) ->  
+  max_value f' P' t.
+Proof.
+  unfold max_value; ins; desf; splits; ins.
+  rewrite H1; specialize (H0 a); desf; eauto.
+  exists a_max; rewrite H1; specialize (H0 a_max); desf; split; auto.
+Qed.
 
-Lemma f_equal_max_same_set f rel cap rel' :
-  f_equal_max f rel cap ->
-  (forall x, rel x <-> rel' x) ->  
-  f_equal_max f rel' cap.
+
+
+Lemma max_value_join_if f f' P P' P'' t t' (cond : bool):
+  max_value f P t ->
+  max_value f P' t' ->
+  (forall x, P'' x <-> P x \/ P' x /\ cond) ->
+  (forall x, P'' x -> f' x = f x) ->  
+  max_value f' P'' (Time.join t (if cond then t' else Time.bot)).
+Proof.
+unfold max_value; ins; desf; splits; ins.
+- rewrite H2; rewrite H1 in *; desf;
+  try by etransitivity; eauto; eauto using Time.join_l, Time.join_r. 
+- destruct (Time.le_lt_dec (f a_max) (f a_max0));
+    [exists a_max0|exists a_max];
+  splits; try by (rewrite H1; auto).
+  all: rewrite H2.
+  all: try (apply Time.join_spec; eauto;
+       etransitivity; eauto; rewrite Time.le_lteq; eauto). 
+  all: rewrite H1; eauto.
+- rewrite H2; rewrite H1 in *; desf;
+  try by etransitivity; eauto; eauto using Time.join_l, Time.join_r. 
+- exists a_max0.
+  rewrite H2; rewrite H1; splits; eauto.
+  apply Time.join_spec; eauto using Time.bot_spec.
+Qed.
+
+Lemma max_value_join f f' P P' P'' t t':
+  max_value f P t ->
+  max_value f P' t' ->
+  (forall x, P'' x <-> P x \/ P' x) ->
+  (forall x, P'' x -> f' x = f x) ->  
+  max_value f' P'' (Time.join t t').
 Proof.
 Admitted.
 
-Lemma f_equal_max_join f rel cap rel' cap' rel'' :
-  f_equal_max f rel cap ->
-  f_equal_max f rel' cap' ->
-  (forall x, rel'' x <-> rel x \/ rel' x) ->
-  f_equal_max f rel'' (Time.join cap cap').
-Proof.
-  unfold f_equal_max; ins; desf; splits; ins.
-  rewrite H1 in *; desf; etransitivity; eauto; eauto using Time.join_l, Time.join_r. 
-  destruct (Time.le_lt_dec (f a_max) (f a_max0));
-    [exists a_max0|exists a_max]; rewrite H1; split; eauto;
-    apply Time.join_spec; eauto;
-  etransitivity; eauto; rewrite Time.le_lteq; eauto.
-Qed.
-
-
-Lemma f_equal_max_join_if f P t P' t' (cond : bool) P'' :
-  f_equal_max f P t ->
-  f_equal_max f P' t' ->
-  (forall x, P'' x <-> P x \/ P' x /\ cond) ->
-  f_equal_max f P'' (Time.join t (if cond then t' else Time.bot)).
-Proof.
-unfold f_equal_max; ins; desf; splits; ins.
-- rewrite H1 in *; desf; etransitivity; eauto; eauto using Time.join_l, Time.join_r. 
-- destruct (Time.le_lt_dec (f a_max) (f a_max0));
-  [exists a_max0|exists a_max]; rewrite H1; split; eauto;
-  apply Time.join_spec; eauto;
-  etransitivity; eauto; rewrite Time.le_lteq; eauto.
-- rewrite H1 in *; desf; etransitivity; eauto; eauto using Time.join_l, Time.join_r. 
-- exists a_max0.
-  rewrite H1; splits; eauto.
-  apply Time.join_spec; eauto using Time.bot_spec.
-Qed.
-
-Lemma f_equal_max_join_if2 f P t P' t' (pred:Prop) (cond : {pred} + {~pred}) P'' :
-  f_equal_max f P t ->
-  f_equal_max f P' t' ->
+Lemma max_value_join_if2 f f' P P' P'' t t' (pred:Prop) (cond : {pred} + {~pred}):
+  max_value f P t ->
+  max_value f P' t' ->
   (forall x, P'' x <-> P x \/ P' x /\ pred) ->
-  f_equal_max f P'' (Time.join t (if cond then t' else Time.bot)).
+  (forall x, P'' x -> f' x = f x) ->  
+  max_value f' P'' (Time.join t (if cond then t' else Time.bot)).
 Proof.
-unfold f_equal_max; ins; desf; splits; ins.
-- rewrite H1 in *; desf; etransitivity; eauto; eauto using Time.join_l, Time.join_r. 
+unfold max_value; ins; desf; splits; ins.
+- rewrite H2; rewrite H1 in *; desf;
+  try by etransitivity; eauto; eauto using Time.join_l, Time.join_r. 
 - destruct (Time.le_lt_dec (f a_max) (f a_max0));
-  [exists a_max0|exists a_max]; rewrite H1; split; eauto;
-  apply Time.join_spec; eauto;
-  etransitivity; eauto; rewrite Time.le_lteq; eauto.
-- rewrite H1 in *; desf; etransitivity; eauto; eauto using Time.join_l, Time.join_r. 
+    [exists a_max0|exists a_max];
+  splits; try by (rewrite H1; auto).
+  all: rewrite H2.
+  all: try (apply Time.join_spec; eauto;
+       etransitivity; eauto; rewrite Time.le_lteq; eauto). 
+  all: rewrite H1; eauto.
+- rewrite H2; rewrite H1 in *; desf;
+  try by etransitivity; eauto; eauto using Time.join_l, Time.join_r. 
 - exists a_max0.
-  rewrite H1; splits; eauto.
+  rewrite H2; rewrite H1; splits; eauto.
   apply Time.join_spec; eauto using Time.bot_spec.
 Qed.
- 
+
 
 (* Lemma my_Time_join_l a b c:
 Time.le a b ->
@@ -305,24 +337,50 @@ Proof.
 reflexivity.
 Qed. *)
 
-Lemma f_equal_max_join_if_loc f P P' t t' (cond : bool) l l' b P'':
-  f_equal_max f P t ->
-  f_equal_max f P' t' ->
-  (forall x, P'' x <-> P x \/ (eq b) x /\ l=l' \/ P' x /\ cond) ->
-f_equal_max f P''
+(* max_value f'
+  (t_cur urr (acts ax_st') (sb ax_st') (rmw ax_st') (rf ax_st') (sc ax_st') (thread a) l')
+  (Time.join (Capability.ur (Commit.cur (Local.commit local)) l')
+     (if LocSet.Facts.eq_dec l l' then f' a else Time.bot))
+ *)
+Lemma max_value_join_loc f f' P P' t l l' b (LOC: loc b = Some l):
+  max_value f P t ->
+  (forall x, P' x <-> P x \/ x = b /\ loc x = Some l') ->
+  (forall x, P x -> f' x = f x) ->  
+  max_value f' P'
+  (Time.join t
+     (if LocSet.Facts.eq_dec l l' then (f' b) else Time.bot)).
+Proof.
+ins.
+eapply max_value_join_if2 with (f:=f'); eauto.
+eapply max_value_same_set; eauto.
+apply max_value_singleton; eauto.
+intro; specialize (H1 x); specialize (H0 x).
+split; ins; desf; eauto.
+apply H0 in H2; desf; eauto.
+Qed.
+
+Lemma max_value_join_if_loc f f' P P' P'' t t' (cond : bool) l l' b (LOC: loc b = Some l):
+  max_value f P t ->
+  max_value f P' t' ->
+  (forall x, P'' x <-> P x \/ P' x /\ cond \/ x = b /\ loc x = Some l') ->
+  (forall x, P' x -> f' x = f x) ->  
+  (forall x, P x -> f' x = f x) ->  
+  max_value f' P''
   (Time.join (Time.join t
-     (if LocSet.Facts.eq_dec l l' then (f b) else Time.bot))
+     (if LocSet.Facts.eq_dec l l' then (f' b) else Time.bot))
      (if cond then t' else Time.bot)).
 Proof.
 ins.
-eapply f_equal_max_join_if with(P:= fun x=>P x \/ b = x /\ l = l'); 
+eapply max_value_join_if with (f:=f') (P:= fun x=>P x \/ b = x /\ l = l') (P':=P'); 
 try edone.
-eapply f_equal_max_join_if2; try edone.
-apply f_equal_max_singleton.
-eauto.
-intro; specialize (H1 x); tauto.
+- eapply max_value_join_if2 with (f:=f'); eauto.
+eapply max_value_same_set; eauto.
+apply max_value_singleton; eauto.
+- eapply max_value_same_set; eauto.
+- intro; specialize (H1 x).
+split; ins; desf; eauto.
+apply H1 in H4; desf; eauto.
 Qed.
-
 
 Lemma sim_local_other_threads acts sb rmw rf mo sc acts' sb' rmw' rf' mo' sc'
   a (GSTEP: gstep acts sb rmw rf mo sc acts' sb' rmw' rf' mo' sc' a)
@@ -331,40 +389,65 @@ Lemma sim_local_other_threads acts sb rmw rf mo sc acts' sb' rmw' rf' mo' sc'
     sim_local f acts' sb' rmw' rf' sc' local i.
 Proof.
 unfold sim_local, sim_commit, sim_cur, sim_acq, sim_rel in *; desf; splits;
-ins; eapply f_equal_max_same_set; try edone; intro.
-- unfold t_cur; unfold dom_rel;
-  split; ins; desc; eexists; [eapply gstep_c_cur_other | 
-  eapply gstep_c_cur_other with (tm':=urr acts' sb' rmw' rf' sc')]; 
-  eauto using gstep_urr_a, urr_mon.
-- unfold t_cur; unfold dom_rel;
-  split; ins; desc; eexists; [eapply gstep_c_cur_other | 
-  eapply gstep_c_cur_other with (tm':=rwr acts' sb' rmw' rf' sc')]; 
-  eauto using gstep_rwr_a, rwr_mon.
-- unfold t_cur; unfold dom_rel;
-  split; ins; desc; eexists; [eapply gstep_c_cur_other | 
-  eapply gstep_c_cur_other with (tm':=scr acts' sb' rmw' rf' sc')]; 
-  eauto using gstep_scr_a, scr_mon.
-- unfold t_acq; unfold dom_rel;
-  split; ins; desc; eexists; [eapply gstep_c_acq_other | 
-  eapply gstep_c_acq_other with (tm':=urr acts' sb' rmw' rf' sc')]; 
-  eauto using gstep_urr_rel_a, urr_mon.
-- unfold t_acq; unfold dom_rel;
-  split; ins; desc; eexists; [eapply gstep_c_acq_other | 
-  eapply gstep_c_acq_other with (tm':=rwr acts' sb' rmw' rf' sc')]; 
-  eauto using gstep_rwr_a, rwr_mon.
-- unfold t_acq; unfold dom_rel;
-  split; ins; desc; eexists; [eapply gstep_c_acq_other | 
-  eapply gstep_c_acq_other with (tm':=scr acts' sb' rmw' rf' sc')]; 
-  eauto using gstep_scr_a, scr_mon.
+ins; eapply max_value_same_set; try edone; intro; symmetry.
+all: try eapply gstep_t_cur_other;  
+     try eapply gstep_t_acq_other;  
+     try eapply gstep_t_rel_other;  
+     eauto 2 using gstep_urr_a, gstep_rwr_a, gstep_scr_a, urr_mon, rwr_mon, scr_mon.
+Qed.
 
-
-Admitted.
-
-Lemma Readable_cur_urr acts sb rmw rf mo sc acts' sb' rmw' rf' mo' sc'
+Lemma sim_local_other_threads' acts sb rmw rf mo sc acts' sb' rmw' rf' mo' sc'
   a (GSTEP: gstep acts sb rmw rf mo sc acts' sb' rmw' rf' mo' sc' a)
   (COH: Coherent acts sb rmw rf mo sc) 
-  t f (VALID: valid f mo) l v o b (LABa: lab a = Aload l v o)
-  (CUR: f_equal_max f (t_cur urr acts sb rmw rf sc (thread a) l) t) 
+  f f' i (NEQ: i <> thread a) local 
+  (LOCAL: sim_local f acts sb rmw rf sc local i)
+  (F: forall a, (In a acts) -> f' a = f a) :
+    sim_local f' acts' sb' rmw' rf' sc' local i.
+Proof.
+unfold sim_local, sim_commit, sim_cur, sim_acq, sim_rel in *; desf; splits;
+ins; eapply max_value_same_set; try edone; intro; symmetry.
+all: try eapply gstep_t_cur_other;  
+     try eapply gstep_t_acq_other;  
+     try eapply gstep_t_rel_other;  
+     eauto 2 using gstep_urr_a, gstep_rwr_a, gstep_scr_a, urr_mon, rwr_mon, scr_mon.
+all: symmetry; apply F; eauto with acts.
+Qed.
+
+Lemma gstep_tm_to_a acts sb rmw rf mo sc acts' sb' rmw' rf' mo' sc'
+  a (GSTEP: gstep acts sb rmw rf mo sc acts' sb' rmw' rf' mo' sc' a)
+  (COH: Coherent acts sb rmw rf mo sc) 
+  tm 
+  (TM_HB: inclusion (tm acts' sb' rmw' rf' sc' ;; hb acts' sb' rmw' rf') (tm acts' sb' rmw' rf' sc'))
+  (TM_MON: inclusion (tm acts sb rmw rf sc) (tm acts' sb' rmw' rf' sc'))
+  (TM_ACTS : forall x y, tm acts sb rmw rf sc x y -> In y acts)
+   l x (CUR: t_cur tm acts sb rmw rf sc (thread a) l x) :
+   tm acts' sb' rmw' rf' sc' x a.
+Proof.
+red in CUR; red in CUR; desc.
+red in CUR; desc.
+unfold seq, eqv_rel in *.
+desc; subst.
+apply TM_HB; exists y; split.
+apply TM_MON; done.
+apply sb_in_hb; eapply gstep_sb; eauto.
+right; red; repeat (eexists; splits; eauto).
+Qed.
+
+(******************************************************************************)
+(** * Lemmas for the read step   *)
+(******************************************************************************)
+
+Lemma Readable_cur_tm acts sb rmw rf mo sc acts' sb' rmw' rf' mo' sc'
+  a (GSTEP: gstep acts sb rmw rf mo sc acts' sb' rmw' rf' mo' sc' a)
+  (COH: Coherent acts sb rmw rf mo sc) 
+  t f (MON: monotone mo f) l v o b (LABa: lab a = Aload l v o)
+  tm (CUR: max_value f (t_cur tm acts sb rmw rf sc (thread a) l) t) 
+  (WRITE : forall x, t_cur tm acts sb rmw rf sc (thread a) l x -> is_write x)
+  (ACTS : forall x, t_cur tm acts sb rmw rf sc (thread a) l x -> In x acts)
+  (COHERENT: forall c, mo' b c -> tm acts' sb' rmw' rf' sc' c a -> False)
+  (TM_HB: inclusion (tm acts' sb' rmw' rf' sc' ;; hb acts' sb' rmw' rf') (tm acts' sb' rmw' rf' sc'))
+  (TM_MON: inclusion (tm acts sb rmw rf sc) (tm acts' sb' rmw' rf' sc'))
+  (TM_ACTS : forall x y, tm acts sb rmw rf sc x y -> In y acts)
   (RFb: rf' b a) : Time.le t (f b).
 Proof.
 assert (~ is_write a).
@@ -372,166 +455,403 @@ assert (~ is_write a).
 red in CUR; desf.
 eapply transitivity with (y:=f a_max); try done.
 cdes GSTEP. 
-eapply valid_converse with (acts:=(a :: acts)); eauto.
-- right. admit. (* red in INa. red in INa. desf. red in INa. eauto with rel. eapply c_cur_ur_in_acts; eauto.*)
+eapply monotone_converse with (acts:=(a :: acts)); eauto.
+- right; eauto. 
 - eapply rf_acta in RFb; eauto. rewrite <- ACT_STEP; eauto.
-- admit. (* eapply c_cur_ur_dom1; eauto.*)
 - eapply rf_doma in RFb; eauto.
 - red in INa; red in INa; desc. apply c_cur_doma2 in INa. edone.
 - eapply loceq_rf in RFb; eauto. unfold loc in *. rewrite LABa in RFb. done.
-- cdes COH0; cdes WF; cdes WF_MO; eauto.
-  intro; rewrite gstep_non_write_mo with (mo':=mo'); eauto.
-  rewrite <- ACT_STEP; eauto.
+- rewrite gstep_non_write_mo with (mo':=mo'); eauto.
+  rewrite <- ACT_STEP.
+  cdes COH0; cdes WF; eauto.
 - intro.
-eapply Coherent_ur with (mo:=mo') (c:=a); eauto.
-eapply gstep_non_write_mo with (acts:=acts) (mo:=mo); eauto.
-(*     eby eapply gstep_new_ur0 with (acts:=acts) (a:=a). 
- *)
-Admitted.
-
-Lemma Readable_cur_rwr acts sb rmw rf mo sc acts' sb' rmw' rf' mo' sc'
-  a (GSTEP: gstep acts sb rmw rf mo sc acts' sb' rmw' rf' mo' sc' a)
-  (COH: Coherent acts sb rmw rf mo sc) 
-  t f (VALID: valid f mo) l v o b (LABa: lab a = Aload l v o)
-  (CUR: f_equal_max f (t_cur rwr acts sb rmw rf sc (thread a) l) t) 
-  (RFb: rf' b a) (RLX: is_rlx a): Time.le t (f b).
-Proof.
-Admitted.
-
-Lemma Readable_cur_scr acts sb rmw rf mo sc acts' sb' rmw' rf' mo' sc'
-  a (GSTEP: gstep acts sb rmw rf mo sc acts' sb' rmw' rf' mo' sc' a)
-  (COH: Coherent acts sb rmw rf mo sc) 
-  t f (VALID: valid f mo) l v o b (LABa: lab a = Aload l v o)
-  (CUR: f_equal_max f (t_cur scr acts sb rmw rf sc (thread a) l) t) 
-  (RFb: rf' b a) (SC: is_sc a): Time.le t (f b).
-Proof.
-Admitted.
+  eapply COHERENT; eauto.
+  eapply gstep_non_write_mo with (acts:=acts) (mo:=mo); eauto.
+  eapply gstep_tm_to_a; eauto.
+Qed.
 
 Lemma Readable_msg_sc acts sb rmw rf mo sc acts' sb' rmw' rf' mo' sc'
   a (GSTEP: gstep acts sb rmw rf mo sc acts' sb' rmw' rf' mo' sc' a)
   (COH: Coherent acts sb rmw rf mo sc) 
-  t f (VALID: valid f mo) l v o b (LABa: lab a = Aload l v o)
-  (MSG: f_equal_max f (msg_rel scr acts sb rmw rf sc l b) t)
+  t f (MON: monotone mo f) l v o b (LABa: lab a = Aload l v o)
+  (MSG: max_value f (fun a => msg_rel scr acts sb rmw rf sc l a b) t)
   (RFb: rf' b a) (SC: is_sc a): Time.le t (f b).
 Proof.
+assert (~ is_write a).
+  intro; unfold is_write in *; destruct (lab a); ins.
+red in MSG; desf.
+eapply transitivity with (y:=f a_max); try done.
+cdes GSTEP. 
+eapply monotone_converse with (acts:=(a :: acts)); eauto.
+- right; eapply acta_msg_scr; eauto.
+- eapply rf_acta in RFb; eauto. rewrite <- ACT_STEP; eauto.
+- eauto with rel.
+- eapply rf_doma in RFb; eauto.
+- eauto with rel.
+- eapply loceq_rf in RFb; eauto. unfold loc in *. rewrite LABa in RFb. auto.
+- rewrite gstep_non_write_mo with (mo':=mo'); eauto.
+  rewrite <- ACT_STEP.
+  cdes COH0; cdes WF; eauto.
+- intro. red in INa. red in INa.
+  unfold seq, eqv_rel in INa; desc; subst.
+  eapply Coherent_scr_rel; eauto.
+  eapply gstep_non_write_mo with (mo:=mo); eauto.
+  eapply scr_rel_mon; eauto.
+  eexists; eauto.
+Qed.
+
+Lemma Readable_full acts sb rmw rf mo sc acts' sb' rmw' rf' mo' sc'
+  a (GSTEP: gstep acts sb rmw rf mo sc acts' sb' rmw' rf' mo' sc' a)
+  (COH: Coherent acts sb rmw rf mo sc) 
+  f (MON: monotone mo f) l v o b (LABa: lab a = Aload l v o)
+  local rel
+  (MSG: max_value f (fun a : event => msg_rel scr acts sb rmw rf sc l a b)
+        (Capability.sc rel l))
+  (URR: max_value f (t_cur urr acts sb rmw rf sc (thread a) l)
+           (Capability.ur (Commit.cur (Local.commit local)) l))
+  (RWR: max_value f (t_cur rwr acts sb rmw rf sc (thread a) l)
+           (Capability.rw (Commit.cur (Local.commit local)) l))
+  (SCR: max_value f (t_cur scr acts sb rmw rf sc (thread a) l)
+           (Capability.sc (Commit.cur (Local.commit local)) l))
+  (RFb: rf' b a): 
+    Commit.readable (Local.commit local) l (f b) rel o.
+Proof.
+constructor; try intro.
+-  eapply Readable_cur_tm; eauto using Coherent_ur, urr_hb, urr_mon with rel acts.
+   by eapply urr_actb; eauto.
+- eapply Readable_cur_tm; eauto using rwr_hb, rwr_mon with rel acts.
+  ins; eapply Coherent_rw with (mo:=mo'); eauto.
+  right; splits; eauto with acts.
+  eapply rwr_actb; eauto.
+- eapply Readable_cur_tm; eauto using scr_hb, scr_mon with rel acts.
+  ins; eapply Coherent_scr with (mo:=mo');  eauto with acts.
+  eapply scr_actb; eauto.
+- eapply Readable_msg_sc; eauto with acts.
+Qed.
+
+(******************************************************************************)
+(** * Lemmas for the write step   *)
+(******************************************************************************)
+
+Lemma Writable_cur_rwr acts sb rmw rf mo sc acts' sb' rmw' rf' mo' sc'
+  a (GSTEP: gstep acts sb rmw rf mo sc acts' sb' rmw' rf' mo' sc' a)
+  (COH: Coherent acts sb rmw rf mo sc) 
+  t f f' (F : forall b, In b acts -> f' b = f b)
+  (MON: monotone mo' f') l v o (LABa: lab a = Astore l v o)
+  (CUR: max_value f (t_cur rwr acts sb rmw rf sc (thread a) l) t) 
+   : Time.lt t (f' a).
+Proof.
+red in CUR; desf.
+eapply TimeFacts.le_lt_lt with (b:=f a_max); try done.
+cdes GSTEP.
+rewrite <- F; eauto with acts.
+eapply monotone_converse_strict with (acts:=(a :: acts)); eauto.
+- right; eauto with acts. 
+- left; done.
+- eauto with rel.
+- eauto with acts. 
+- eauto with rel.
+- unfold loc; rewrite LABa; done.
+- rewrite <- ACT_STEP.
+  cdes COH0; cdes WF; eauto.
+- intro.
+  eapply Coherent_rw; eauto.
+  eapply gstep_tm_to_a; eauto.
+  eapply rwr_hb.
+  eapply rwr_mon; eauto.
+  eapply rwr_actb; eauto.
+- intro; subst; eauto with acts. 
+Qed.
+
+Lemma Writable_cur_scr acts sb rmw rf mo sc acts' sb' rmw' rf' mo' sc'
+  a (GSTEP: gstep acts sb rmw rf mo sc acts' sb' rmw' rf' mo' sc' a)
+  (COH: Coherent acts sb rmw rf mo sc) 
+  t f f' (F : forall b, In b acts -> f' b = f b)
+  (MON: monotone mo' f') l v o (LABa: lab a = Astore l v o)
+  (CUR: max_value f (t_cur scr acts sb rmw rf sc (thread a) l) t) 
+  (SC: is_sc a) : Time.lt t (f' a).
+Proof.
+red in CUR; desf.
+eapply TimeFacts.le_lt_lt with (b:=f a_max); try done.
+cdes GSTEP.
+rewrite <- F; eauto with acts.
+eapply monotone_converse_strict with (acts:=(a :: acts)); eauto.
+- right; eauto with acts. 
+- left; done.
+- eauto with rel.
+- eauto with acts. 
+- eauto with rel.
+- unfold loc; rewrite LABa; done.
+- rewrite <- ACT_STEP.
+  cdes COH0; cdes WF; eauto.
+- intro.
+  eapply Coherent_scr; eauto.
+  eapply gstep_tm_to_a; eauto.
+  eapply scr_hb.
+  eapply scr_mon; eauto.
+  eapply scr_actb; eauto.
+- intro; subst; eauto with acts. 
+Qed.
+
+Lemma Writable_sc_map acts sb rmw rf mo sc acts' sb' rmw' rf' mo' sc'
+  a (GSTEP: gstep acts sb rmw rf mo sc acts' sb' rmw' rf' mo' sc' a)
+  (COH: Coherent acts sb rmw rf mo sc) 
+  t f f' (F : forall b, In b acts -> f' b = f b)
+  (MON: monotone mo' f') l v o (LABa: lab a = Astore l v o)
+  (SCMAP: max_value f (S_tm acts sb rmw rf l) t)
+  (SC: is_sc a) : Time.lt t (f' a).
+Proof.
+red in SCMAP; desf.
+eapply TimeFacts.le_lt_lt with (b:=f a_max); try done.
+cdes GSTEP.
+rewrite <- F; eauto with acts.
+eapply monotone_converse_strict with (acts:=(a :: acts)); eauto.
+- right; eauto with acts. 
+- left; done.
+- eauto with rel.
+- eauto with acts. 
+- eauto with rel.
+- unfold loc; rewrite LABa; done.
+- rewrite <- ACT_STEP.
+  cdes COH0; cdes WF; eauto.
+- intro.
+  eapply Coherent_scr; eauto.
+  red in INa; red in INa; desc.
+  eapply S_tm_sc; eauto with acts.
+  eapply S_tmr_mon; eauto.
+Qed.
+
+Lemma Writable_full acts sb rmw rf mo sc acts' sb' rmw' rf' mo' sc'
+  a (GSTEP: gstep acts sb rmw rf mo sc acts' sb' rmw' rf' mo' sc' a)
+  (COH: Coherent acts sb rmw rf mo sc) 
+  f f' (F : forall b, In b acts -> f' b = f b)
+  (MON: monotone mo' f')
+  l v o (LABa: lab a = Astore l v o)
+  local sc_map
+  (SC : forall l : Loc.t, max_value f (S_tm acts sb rmw rf l) (sc_map l))
+  (RWR: max_value f (t_cur rwr acts sb rmw rf sc (thread a) l)
+           (Capability.rw (Commit.cur (Local.commit local)) l))
+  (SCR: max_value f (t_cur scr acts sb rmw rf sc (thread a) l)
+           (Capability.sc (Commit.cur (Local.commit local)) l)):
+  Commit.writable (Local.commit local) sc_map l (f' a) o.
+Proof.
+constructor; try intro.
+eapply Writable_cur_rwr; eauto.
+eapply Writable_cur_scr; eauto with acts.
+eapply Writable_sc_map; eauto with acts.
 Admitted.
 
-Lemma ax_op_sim :
-  forall op_st ax_st (SIM: sim op_st ax_st) ax_st' (AXSTEP: m_step ax_st ax_st'),
-  exists op_st' e tid, Configuration.step e tid op_st op_st' /\ sim op_st' ax_st'.
-Proof.
-destruct ax_st, ax_st'; ins.
-destruct AXSTEP; ins.
-unfold sim, sim_f in SIM; ins; desf.
-apply find_mapD in TID; desc; destruct z as [? local]; ins; desf.
-
-generalize (gstep_read_rf COH GSTEP LAB_STEP); intro; desc.
-
-assert (NON_WRITE: ~ is_write a).
-  unfold is_write; destruct (lab a); ins.
-generalize (gstep_non_write_mo COH GSTEP NON_WRITE) as SAME_MO; intro; desc.
-rewrite SAME_MO in *. 
-clear NON_WRITE.
-
-assert (E: exists from rel, Cell.get (f b) ((Configuration.memory op_st) l) = 
-          Some (from, {| Message.val:=v; Message.released:=rel |})).
-  cdes GSTEP; cdes INC; cdes COH0; cdes WF.
-  eapply get_cell; try edone; rewrite <- ACT_STEP in *; try edone.
-
-assert (RA: is_ra a = Ordering.le Ordering.acqrel o).
-unfold is_ra, is_ra_lab; rewrite LAB_STEP; done.
-
-assert (RLX: is_rlx a = Ordering.le Ordering.relaxed o).
-unfold is_rlx, is_rlx_lab; rewrite LAB_STEP; done.
-
-
-assert (WRITE_B: is_write b). 
-  unfold is_write; destruct (lab b); ins.
-
-assert (LOC_B: loc b = Some l). 
-  unfold loc; destruct (lab b); ins; desf.
-
-
-cdes MEM.  
-specialize (MEM l). 
-red in MEM; desc.
-specialize (SIMCELL b WRITE_B LOC_B from {| Message.val := v; Message.released := rel |} E).
-red in SIMCELL; desc; red in SIMMSG; desc.
-
-desf.
-
-assert (READABLE: Commit.readable (Local.commit local) l (f b) rel o).
-{
-  specialize (LOCAL (thread a) (existT _ lang st) local TID); desf.
-  red in LOCAL; red in LOCAL; desc; red in CUR; desc.
-  constructor.
-  - specialize (CUR_UR l); eapply Readable_cur_urr; eauto.
-  - specialize (CUR_RW l). intro. 
-    eapply Readable_cur_rwr; eauto.
-    unfold is_rlx; rewrite LAB_STEP; ins.
-  - specialize (CUR_SC l). intro. 
-    eapply Readable_cur_scr; eauto.
-    unfold is_sc; rewrite LAB_STEP; ins.
-  - specialize (SC0 l). intro. 
-    eapply Readable_msg_sc; eauto.
-    unfold is_sc; rewrite LAB_STEP; ins.
-}
-
-eexists _,_,(thread a).
+(******************************************************************************)
+(** * Main Theorem: the operational machine simulates the axiomatic machine   *)
+(******************************************************************************)
 
 Lemma foo (P Q : Prop) : P -> (P -> Q) -> P /\ Q.
 Proof. tauto. Qed.
 
+Lemma ax_op_sim_helper 
+op_st ax_st (SIM: sim op_st ax_st) ax_st' (AXSTEP: step ax_st ax_st')
+(NEXT: exists (e0 : option Event.t) (tid : Ident.t) threads sc_map memory,
+  Configuration.step e0 tid op_st 
+    {| Configuration.threads:=threads; Configuration.sc:=sc_map; 
+       Configuration.memory:=memory  |}
+  /\
+  sim {| Configuration.threads:=threads; Configuration.sc:=sc_map; 
+         Configuration.memory:=memory  |} ax_st') :
+  exists e tid op_st', Configuration.step e tid op_st op_st' /\ sim op_st' ax_st'.
+Proof.
+desf.
+eauto.
+Qed.
+
+Lemma ax_op_sim :
+  forall op_st ax_st (SIM: sim op_st ax_st) ax_st' (AXSTEP: step ax_st ax_st'),
+  exists e tid op_st', Configuration.step e tid op_st op_st' /\ sim op_st' ax_st'.
+Proof.
+ins.
+destruct AXSTEP.
+red in SIM; desc.
+red in SIM. desc. 
+rewrite STATES in TID.
+apply find_mapD in TID; desc; destruct z as [? local]; ins; desf.
+
+destruct MSTEP; subst.
+
+(** SILENT **)
+{
+eexists _,i,_.
+split.
+econstructor; try edone.
+eauto.
+apply Thread.step_program.
+eapply Thread.step_silent; edone.
+admit.
+admit.
+}
+
+(** READ **)
+{
+assert (SCa: is_sc a = Ordering.le Ordering.seqcst o).
+  unfold is_sc; unfold ord; rewrite LABa; done.
+assert (RAa: is_ra a = Ordering.le Ordering.acqrel o).
+  unfold is_ra; unfold ord; rewrite LABa; done.
+assert (RLXa: is_rlx a = Ordering.le Ordering.relaxed o).
+  unfold is_rlx; unfold ord; rewrite LABa; done.
+
+generalize (gstep_read_rf COH GSTEP LABa); intro; desc.
+
+assert (~ is_wfence a /\ ~ is_write a).
+  unfold is_write, is_wfence; destruct (lab a); ins.
+
+assert (E: exists from rel, Cell.get (f b) ((Configuration.memory op_st) l) = 
+          Some (from, {| Message.val:=v; Message.released:=rel |})).
+  cdes GSTEP; cdes INC; cdes COH0; cdes WF.
+  eapply get_cell; try edone. 
+  rewrite <- ACT_STEP in *; try edone.
+
+assert (WRITE_B: is_write b). 
+  unfold is_write; destruct (lab b); ins.
+assert (LOC_B: Gevents.loc b = Some l). 
+  unfold Gevents.loc; destruct (lab b); ins; desf.
+
+cdes MEM. specialize (MEM l); red in MEM; desc.
+specialize (SIMCELL b WRITE_B LOC_B from 
+  {| Message.val := v; Message.released := rel |} E).
+red in SIMCELL; desc; red in SIMMSG; desc.
+
+eexists _,(thread a),_.
 apply foo; [|intro STEP].
 {
 econstructor; try edone.
-- econstructor.
-- apply Thread.step_program.
+eauto.
+apply Thread.step_program; try edone.
   eapply Thread.step_read; eauto.
-  econstructor; edone.
-- admit.
+  econstructor; try edone.
+  specialize (LOCAL (thread a) (existT _ lang st) local TID); desf.
+  red in LOCAL; red in LOCAL; desc; red in CUR; desc.
+  eapply Readable_full; eauto.
+admit.
+}
+red; simpl; splits; eauto.
+- eby eapply Configuration.step_future.
+- eby eapply Configuration.step_future.
+- ins; rewrite IdentMap.gsspec in TID0; desf; ins;
+  eapply NO_PROMISES; edone.
+- rewrite IdentMap.map_add. admit.
+- clear STEP.
+
+exists f; split.
+* rewrite <- gstep_non_write_mo; eauto with acts.
+* red; splits; ins.
+  + ins; rewrite IdentMap.gsspec in TID0; desf; ins.
+    Focus 2. by eapply sim_local_other_threads; eauto.
+    red; ins; red; ins.
+    exploit LOCAL; clear LOCAL; eauto; intro LOCAL; unfold sim_local in *; ins.
+    unfold sim_commit, sim_acq, sim_cur, sim_rel in *; desc; splits; intro l';
+    simpl;
+    unfold TimeMap.bot.
+    all: try (rewrite !tm_join; rewrite time_join_bot).
+    all: try (rewrite !tm_join; rewrite tm_join_singleton_to_if).
+    all: try rewrite !time_join_bot.
+    all: try rewrite !fun_if; simpl.
+    all: try rewrite !if_arg with (x := l'); simpl.
+    all: unfold TimeMap.bot; simpl.
+    all: try intro; try eapply max_value_join_if_loc; try edone; simpl.
+    all: try intro; try eapply max_value_join_if; try edone.
+    all: try intro; try eapply max_value_same_set; try edone.
+    all: try rewrite <- RAa; try rewrite <- RLXa; try rewrite <- SCa.
+
+
+
+    eapply gstep_t_cur_urr_read; eauto.
+    eapply gstep_t_cur_rwr_read; eauto.
+    eapply gstep_t_cur_scr_read; eauto.
+    eapply gstep_t_acq_urr_read; eauto.
+    admit.
+    admit.
+    intro; symmetry; eapply gstep_t_rel_other; eauto using gstep_urr_a, urr_mon.
+    intro; symmetry; eapply gstep_t_rel_other; eauto using gstep_rwr_a, rwr_mon.
+    intro; symmetry; eapply gstep_t_rel_other; eauto using gstep_scr_a, scr_mon.
++ eapply max_value_same_set; try edone.
+admit.
++ admit.
 }
 
-(* match goal with |- Configuration.step ?G (thread a) op_st ?G' /\ _ =>
-  set (M := G); set (M' := G') end.
- *)
-(* match goal with |- ?G /\ _ =>
-  set (M := G) end.
- *) 
 
+(** Write **)
+{
+generalize (new_f GSTEP MONOTONE); intro; desc.
+
+assert (LOC_A: Gevents.loc a = Some l). 
+  unfold Gevents.loc; destruct (lab a); ins; desf.
+
+
+eexists _,(thread a),_.
+apply foo; [|intro STEP].
+{
+econstructor; try edone.
+eauto.
+apply Thread.step_program; try edone.
+eapply Thread.step_write with (to:= f' a); eauto.
+econstructor; try edone.
+specialize (LOCAL (thread a) (existT _ lang st) local TID); desf.
+red in LOCAL; red in LOCAL; desc; red in CUR; desc.
+eapply Writable_full; eauto.
+admit.
+admit.
+admit.
+}
 
 red; simpl; splits; eauto.
 - eby eapply Configuration.step_future.
 - eby eapply Configuration.step_future.
 - ins; rewrite IdentMap.gsspec in TID0; desf; ins;
   eapply NO_PROMISES; edone.
-- by rewrite IdentMap.map_add.
-- exists f; split; [by apply MONOTONE|].
-  clear STEP; red; splits; ins.
-  * ins; rewrite IdentMap.gsspec in TID0; desf; ins.
-    Focus 2. by eapply sim_local_other_threads; eauto.
-red; ins; red; ins.
-exploit LOCAL; clear LOCAL; eauto; intro LOCAL; unfold sim_local in *; ins.
-unfold sim_commit, sim_acq, sim_cur, sim_rel in *; desc; splits; intro l';
-simpl;
-unfold TimeMap.bot.
-all: try (rewrite !tm_join; rewrite time_join_bot).
-all: try (rewrite !tm_join; rewrite tm_join_singleton_to_if).
-all: try rewrite !time_join_bot.
-all: try rewrite !fun_if; simpl.
-all: try rewrite !if_arg with (x := l'); simpl.
-all: unfold TimeMap.bot; simpl.
-all: try intro; try eapply f_equal_max_join_if_loc; try edone; simpl.
-all: try intro; try eapply f_equal_max_join_if; try edone.
-all: try intro; try eapply f_equal_max_same_set; try edone.
-all: try rewrite <- RA.
-all: try rewrite <- RLX.
+- rewrite IdentMap.map_add. admit.
+-
+  exists f'; splits; try done.
+   red; splits; ins.
+  + ins; rewrite IdentMap.gsspec in TID0; desf; ins.
+    Focus 2.  eapply sim_local_other_threads'; eauto.
+    red; ins; red; ins.
+    exploit LOCAL; clear LOCAL; eauto; intro LOCAL; unfold sim_local in *; ins.
+    unfold sim_commit, sim_acq, sim_cur, sim_rel in *; desc; splits; intro l';
+    simpl.
+    all: unfold TimeMap.bot, LocFun.add; simpl.
+    all: try (rewrite !tm_join; rewrite time_join_bot).
+    all: try (rewrite !tm_join; rewrite tm_join_singleton_to_if).
+    all: try rewrite !time_join_bot.
+    all: try rewrite !fun_if; simpl.
+    all: try rewrite !if_arg with (x := l'); simpl.
+    all: unfold TimeMap.bot; simpl.
+all: try rewrite !if_same.
+    all: try rewrite !time_join_bot.
 
 
-clear -GSTEP LAB_STEP RFb.
+all: try eapply max_value_join_loc; eauto with acts; simpl.
+
+    all: try intro; try eapply max_value_join_if_loc; eauto with acts; simpl.
+    all: try intro; try eapply max_value_join_if; eauto with acts; simpl.
+
+
+    all: try intro; try eapply max_value_same_set; try edone.
+    all: try rewrite <- RAa; try rewrite <- RLXa; try rewrite <- SCa.
+    eapply gstep_t_cur_urr_write; eauto.
+    eapply gstep_t_cur_rwr_read; eauto.
+    eapply gstep_t_cur_scr_read; eauto.
+    eapply gstep_t_acq_urr_read; eauto.
+    admit.
+    admit.
+    intro; symmetry; eapply gstep_t_rel_other; eauto using gstep_urr_a, urr_mon.
+    intro; symmetry; eapply gstep_t_rel_other; eauto using gstep_rwr_a, rwr_mon.
+    intro; symmetry; eapply gstep_t_rel_other; eauto using gstep_scr_a, scr_mon.
++ eapply max_value_same_set; try edone.
+admit.
++ admit.
+
+
+
+}
 Admitted.
-Qed.
-
 
 Lemma ax_sim_op :
   forall op_st ax_st (SIM: sim op_st ax_st) op_st' e tid (OPSTEP: Configuration.step tid e op_st op_st'),
